code/experimental/sha2/Hacl.SHA2_256.fst
@@ -22,19 +22,6 @@ module Impl = Hacl.Impl.SHA2_256
 ///
 
 
-val pad:
-    blocks: lbuffer uint8 (2 * Spec.size_block Spec.SHA2_256)
-  -> prev: uint64
-  -> last: buffer uint8
-  -> len: size_t{ v len == length last
-               /\ v len <= Spec.size_block Spec.SHA2_256
-               /\ v len + uint_v prev <= Spec.max_input Spec.SHA2_256} ->
-  Stack unit
-  (requires (fun h -> live h blocks /\ live h last /\ disjoint blocks last))
-  (ensures  (fun h0 _ h1 -> modifies1 blocks h0 h1))
-
-let pad blocks prev last len = Impl.pad blocks prev last len
-
 val init: hash:lbuffer uint32 8 ->
   Stack unit
   (requires (fun h -> live h hash))
@@ -71,7 +58,7 @@ val update:
     hash: lbuffer uint32 8
   -> input: buffer uint8
   -> len: size_t{ v len == length input
-               /\ v len <= pow2 61} ->
+               /\ v len <= pow2 61 - 1} ->
   Stack unit
   (requires (fun h -> live h hash /\ live h input /\ disjoint hash input))
   (ensures  (fun h0 _ h1 -> modifies1 hash h0 h1))
@@ -92,7 +79,7 @@ let finish hash hw = Impl.finish hash hw
 val hash:
     output: lbuffer uint8 32
   -> input: buffer uint8
-  -> len: size_t{length input == v len} ->
+  -> len: size_t{length input == v len /\ v len <= pow2 61 - 1} ->
   Stack unit
   (requires (fun h -> live h output /\ live h input /\ disjoint output input))
   (ensures  (fun h0 _ h1 -> modifies1 output h0 h1))
